CellularAutomatas/proofs/two_stage_is_rt_closed.lean
@@ -92,24 +92,24 @@ theorem two_stage_is_weak_rt_closed (adv: TwoStageAdvice α Γ):
         rw [elemL_iff_trace_rt (by simp)]
         simp [combined, h_empty]
 
-def TwoStageAdvice.liftAdvice (adv: TwoStageAdvice α Γ) (S: Type) [Alphabet S]: TwoStageAdvice (α × S) Γ where
+def TwoStageAdvice.liftAdvice (adv: TwoStageAdvice α Γ) {S: Type} [Alphabet S] (π: S → α): TwoStageAdvice S Γ where
   β := adv.β
-  C := adv.C.map_embed (Option.map Prod.fst)
+  C := adv.C.map_embed (Option.map π)
   M := adv.M
 
-lemma TwoStageAdvice.liftAdvice_advice (adv: TwoStageAdvice α Γ) (S: Type) [Alphabet S]:
-    (adv.liftAdvice S).advice = adv.advice.lift S := by
+lemma TwoStageAdvice.liftAdvice_advice (adv: TwoStageAdvice α Γ) {S: Type} [Alphabet S] (π: S → α):
+    (adv.liftAdvice π).advice = adv.advice.lift π := by
   apply advice_eq_iff
   funext w
   simp only [TwoStageAdvice.liftAdvice, TwoStageAdvice.advice, Function.comp, Advice.lift]
   congr 1
-  exact map_embed_trace_rt adv.C Prod.fst w
+  exact map_embed_trace_rt adv.C π w
 
 theorem two_stage_is_rt_closed (adv: TwoStageAdvice α Γ):
     adv.advice.rt_closed := by
-  intro S _inst
-  rw [← adv.liftAdvice_advice S]
-  exact two_stage_is_weak_rt_closed (adv.liftAdvice S)
+  intro S _inst π
+  rw [← adv.liftAdvice_advice π]
+  exact two_stage_is_weak_rt_closed (adv.liftAdvice π)
 
 theorem cart_is_rt_closed (C: CArtTransducer α Γ):
     C.advice.rt_closed :=
